try some things, remove fractional RA

theories/logrel_heaplang_sessions/examples/double.v
@@ -1,10 +1,11 @@
 From iris.heap_lang Require Export lifting metatheory.
 From iris.base_logic.lib Require Import invariants.
-From iris.heap_lang Require Import notation proofmode lib.par.
+From iris.heap_lang Require Import notation proofmode lib.par lib.spin_lock.
 From iris.algebra Require Import agree frac csum excl.
 From actris.channel Require Import proto_channel channel proofmode.
 
 Definition prog (c : val) : expr :=
+  let: "lock" := newlock #() in
   let: "d1" := new_chan #() in
   let: "d1send" := Fst "d1" in
   let: "d1recv" := Snd "d1" in
@@ -12,35 +13,149 @@ Definition prog (c : val) : expr :=
   let: "d2send" := Fst "d2" in
   let: "d2recv" := Snd "d2" in
   (
+    acquire "lock";;
     let: "x1" := recv c in
+    release "lock";;
     send "d1send" "x1";;
     let: "x2" := recv "d2recv" in
-    if: "x1" ≤ "x2" then send "c" "x1" else Skip
+    if: "x1" ≤ "x2"
+    then acquire "lock";; send "c" "x1";; release "lock"
+    else Skip
   ) ||| (
+    acquire "lock";;
     let: "x2" := recv c in
+    release "lock";;
     send "d2send" "x2";;
     let: "x1" := recv "d1recv" in
-    if: "x2" < "x1" then send "c" "x2" else Skip
+    if: "x2" < "x1"
+    then acquire "lock";; send "c" "x2";; release "lock"
+    else Skip
   ).
 
 Section GhostState.
-  Definition doubleR := fracR.
-  Class doubleG Σ := { double_inG :> inG Σ doubleR }.
-  Definition doubleΣ : gFunctors := #[GFunctor doubleR].
-  Global Instance subG_doubleΣ {Σ} : subG doubleΣ Σ → doubleG Σ.
+  (* one-shot RA, slightly modified from iris-examples *)
+  Definition oneshotR := csumR (exclR unitO) (agreeR natO).
+  Class oneshotG Σ := { oneshot_inG :> inG Σ oneshotR }.
+  Definition oneshotΣ : gFunctors := #[GFunctor oneshotR].
+  Instance subG_oneshotΣ {Σ} : subG oneshotΣ Σ → oneshotG Σ.
   Proof. solve_inG. Qed.
+
+  Definition pending `{oneshotG Σ} γ := own γ (Cinl (Excl tt)).
+  Definition shot `{oneshotG Σ} γ (n : nat) := own γ (Cinr (to_agree n)).
+
+  Lemma new_pending `{oneshotG Σ} : (|==> ∃ γ, pending γ)%I.
+  Proof. by apply own_alloc. Qed.
+
+  Lemma shoot `{oneshotG Σ} (n : nat) γ : pending γ ==∗ shot γ n.
+  Proof.
+    apply own_update.
+      by apply cmra_update_exclusive.
+  Qed.
+
+  Lemma shot_not_pending `{oneshotG Σ} γ n :
+    shot γ n -∗ pending γ -∗ False.
+  Proof.
+    iIntros "Hs Hp".
+    iPoseProof (own_valid_2 with "Hs Hp") as "H".
+    iDestruct "H" as %[].
+  Qed.
+
+  Lemma shot_agree `{oneshotG Σ} γ (n m : nat) :
+    shot γ n -∗ shot γ m -∗ ⌜n = m⌝.
+  Proof.
+    iIntros "Hs1 Hs2".
+    iDestruct (own_valid_2 with "Hs1 Hs2") as %Hfoo.
+    iPureIntro. by apply agree_op_invL'.
+Qed.
 End GhostState.
 
 Section Double.
-  Context `{heapG Σ, proto_chanG Σ, doubleG Σ}.
+  Context `{heapG Σ, proto_chanG Σ, oneshotG Σ}.
 
-  Definition prog_proto : iProto Σ :=
+  Definition proto_begin : iProto Σ :=
     (<?> x1 : nat, MSG #x1; <?> x2 : nat, MSG #x2; <!> MSG #(min x1 x2); END)%proto.
 
-  Lemma wp_prog (c : val):
-    {{{ c ↣ prog_proto }}} prog c {{{ v, RET v; True }}}.
+  Definition chan_begin (c : val) (γ1 γ2 : gname) : iProp Σ :=
+    (c ↣ proto_begin)%I.
+  Definition chan_half1 (c : val) (γ1 γ2 : gname) : iProp Σ :=
+    (∃ x1 : nat, shot γ2 x1 ∗ c ↣ <?> x2 : nat, MSG #x2; <!> MSG #(min x1 x2); END)%I.
+  Definition chan_half2 (c : val) (γ1 γ2 : gname) : iProp Σ :=
+    (∃ x1 : nat, shot γ1 x1 ∗ c ↣ <?> x2 : nat, MSG #x2; <!> MSG #(min x1 x2); END)%I.
+  Definition chan_whole (c : val) (γ1 γ2 : gname) : iProp Σ :=
+    (∃ x1 x2 : nat, shot γ1 x1 ∗ shot γ2 x2 ∗ c ↣ <!> MSG #(min x1 x2); END)%I.
+
+  Definition chan_inv (c : val) (γ1 γ2 : gname) : iProp Σ :=
+    (chan_begin c γ1 γ2 ∨
+     chan_half1 c γ1 γ2 ∨
+     chan_half2 c γ1 γ2 ∨
+     chan_whole c γ1 γ2)%I.
+
+  Lemma wp_prog (N : namespace) (c : val):
+    {{{ c ↣ proto_begin }}} prog c {{{ v, RET v; True }}}.
   Proof.
     iIntros (Φ) "Hc HΦ".
+    rewrite /prog.
+
+    iMod new_pending as (γ1) "Hγ1".
+    iMod new_pending as (γ2) "Hγ2".
+
+    (* Create lock *)
+    wp_apply (newlock_spec N (chan_inv c γ1 γ2) with "[Hc]").
+    { iLeft. iFrame "Hc". }
+    iIntros (lk γ) "#Hlock".
+    wp_pures.
+
+    (* Create channel A -> B *)
+    wp_apply new_chan_proto_spec.
+    { done. }
+    iIntros (d1send d1recv) "Hd1".
+    iDestruct ("Hd1" $! (<!> x : nat, MSG #x {{ shot γ1 x }}; END)%proto) as ">[Hd1send Hd1recv]".
+    wp_pures.
+
+    (* Create channel B -> A *)
+    wp_apply new_chan_proto_spec.
+    { done. }
+    iIntros (d2send d2recv) "Hd2".
+    iDestruct ("Hd2" $! (<!> x : nat, MSG #x {{ shot γ2 x }}; END)%proto) as ">[Hd2send Hd2recv]".
+    wp_pures.
+
+    (* Fork into two threads *)
+    wp_apply (wp_par with "[Hd1send Hd2recv Hγ1]").
+
+    - (* Acquire lock *)
+      wp_apply (acquire_spec with "Hlock").
+      iIntros "[Hlocked Hc]". wp_pures.
+      iDestruct "Hc" as "[Hc|[Hc|[Hc|Hc]]]".
+      + wp_apply (recv_proto_spec with "Hc").
+        iIntros (n) "Hc _ /=".
+        wp_pures.
+        iMod (shoot n γ1 with "Hγ1") as "#Hγ1".
+        wp_apply (release_spec with "[Hlock Hlocked Hc Hγ1]").
+        { iFrame "Hlock Hlocked".
+          iRight. iRight. iLeft.
+          iExists n. iFrame "Hγ1 Hc". }
+        iIntros "_". wp_pures.
+
+        (* Send the value to the other thread *)
+        wp_apply (send_proto_spec with "Hd1send").
+        iExists n. iSplit=> //. iSplitR=> //.
+        iModIntro. iIntros "Hd1send /=". wp_pures.
+
+        (* Receive the other thread's value *)
+        wp_apply (recv_proto_spec with "Hd2recv").
+        iIntros (m) "Hd2recv #Hγ2 /=". wp_pures.
+
+        case_bool_decide.
+
+      + admit.
+      + (* Impossible, since this means our one-shot has already been shot *)
+        iDestruct "Hc" as "[Hc _]".
+        iCombine "Hcredit1 Hc" as "Hc".
+        iExFalso.
+        iDestruct (own_valid with "Hc") as %Hvalid.
+        admit.
+      + (* Impossible, since this means our one-shot has already been shot *)
+        admit.
   Admitted.
 
   (* We need to prove using ghost state that at most two receives will
@@ -50,21 +165,4 @@ Section Double.
   invariant needs to ensure that only the process with the lowest
   value can access it. *)
 
-  Definition chan_begin (c : val) (γ1 : gname) : iProp Σ :=
-    (c ↣ <?> x1 : nat, MSG #x1; <?> x2 : nat, MSG #x2; <!> MSG #(min x1 x2); END)%I.
-  Definition chan_half (c : val) (γ1 : gname) : iProp Σ :=
-    ( own γ1 (1/2)%Qp
-    ∗ ∃ x1 : nat, c ↣ <?> x2 : nat, MSG #x2; <!> MSG #(min x1 x2); END)%I.
-  Definition chan_whole (c : val) (γ1 : gname) : iProp Σ :=
-    ( own γ1 1%Qp
-    ∗ ∃ x1 x2 : nat, c ↣ <!> MSG #(min x1 x2); END)%I.
-  Definition chan_done (c : val) (γ1 : gname) : iProp Σ :=
-    ( own γ1 1%Qp
-    ∗ c ↣ END)%I.
-
-  Definition chan_inv (c : val) (γ1 : gname) : iProp Σ :=
-    (chan_begin c γ1 ∨
-     chan_half c γ1 ∨
-     chan_whole c γ1 ∨
-     chan_done c γ1)%I.
 End Double.
